examples/TrivialCache.v
@@ -1,0 +1,163 @@
+Ltac typeof' H := type of H.
+
+Require Import QueryStructureNotations.
+Require Import ListImplementation.
+Require Import AddCache ADTCache.
+
+Definition MySchema :=
+  Query Structure Schema
+    [ relation "Person" has
+          schema <"Age" :: nat,
+                  "Name" :: string>;
+      relation "Dog" has
+          schema <"Owner" :: string,
+                  "Name" :: string,
+                  "Breed" :: string> ]
+    enforcing [].
+
+Definition Person := TupleDef MySchema "Person".
+Definition Dog := TupleDef MySchema "Dog".
+
+Definition MySig : ADTSig :=
+  ADTsignature {
+      "Empty" : unit → rep,
+      "YoungOwners'Breeds" : rep × nat → rep × list string,
+      "BreedPopulation" : rep × string → rep × nat
+  }.
+
+Definition MySpec : ADT MySig :=
+  QueryADTRep MySchema {
+    const "Empty" (_ : unit) : rep := empty,
+
+    query "YoungOwners'Breeds" ( ageLimit : nat ) : list string :=
+      For (d in "Dog")
+          (o in "Person")
+          Where (ageLimit > o!"Age")
+          Where (d!"Name" = o!"Name")
+          Return (d!"Breed"),
+
+    query "BreedPopulation" ( breed : string ) : nat :=
+        Count (For (d in "Dog")
+                   Where (d!"Breed" = breed)
+                   Return ())
+}.
+
+Definition BreedCacheSpec (or : UnConstrQueryStructure MySchema)
+           (cache : string -> nat) :=
+forall breed,
+  refine
+    (Count (For (UnConstrQuery_In or ``("Dog")
+                                  (fun d =>
+                                     Where (d!"Breed" = breed)
+             Return ()))))
+    (ret (cache breed)).
+
+Definition MyListImpl_abs
+           (or : cachedRep (UnConstrQueryStructure MySchema) (string -> nat))
+           (nr : (list Person * list Dog) * (string -> nat)) : Prop :=
+  ((origRep or) ! "Person" ≃ fst (fst nr) /\
+  (origRep or) ! "Dog" ≃ snd (fst nr)) /\
+  cachedVal or = snd nr.
+
+Definition My :
+  Sharpened MySpec.
+Proof.
+  unfold MySpec.
+
+  start honing QueryStructure.
+
+  hone representation using (cachedRep_AbsR BreedCacheSpec).
+
+  hone method "YoungOwners'Breeds".
+  { simplify with monad laws.
+    setoid_rewrite (refine_pick_val _ H0).
+    simplify with monad laws; simpl.
+    unfold cachedRep_AbsR in H0; intuition; subst.
+    finish honing.
+  }
+
+  hone method "BreedPopulation".
+  { simplify with monad laws.
+    setoid_rewrite (refine_pick_val _ H0).
+    simplify with monad laws; simpl.
+    unfold cachedRep_AbsR in H0; intuition; subst.
+    unfold BreedCacheSpec in H2.
+    subst_body.
+    setoid_rewrite (H2 n); simplify with monad laws; simpl.
+    finish honing.
+  }
+
+  hone constructor "Empty".
+  { simplify with monad laws.
+    rewrite refine_pick_cachedRep.
+    rewrite refine_pick_val with (A := string -> nat)
+                                   (a := fun x : string => 0).
+    simplify with monad laws; finish honing.
+    unfold BreedCacheSpec; simpl.
+    intros; setoid_rewrite refine_Count.
+    setoid_rewrite refine_For_In_Empty.
+    simplify with monad laws; reflexivity.
+  }
+
+  hone representation using MyListImpl_abs.
+  hone constructor "Empty".
+  { simplify with monad laws.
+    unfold MyListImpl_abs, GetUnConstrRelation; simpl.
+    rewrite (@refineEquiv_pick_pair_pair
+                  (list Person)
+                  (list Dog)
+                  (string -> nat)
+                  (EnsembleIndexedListEquivalence (fun _ : IndexedTuple => False))
+                  (EnsembleIndexedListEquivalence (fun _ : IndexedTuple => False))
+                  (fun c : string -> nat => (fun _ => 0) = c)).
+    rewrite refine_pick_val by
+        apply EnsembleIndexedListEquivalence_Empty;
+    simplify with monad laws.
+    rewrite refine_pick_val by
+        apply EnsembleIndexedListEquivalence_Empty;
+      simplify with monad laws.
+    rewrite refineEquiv_pick_eq';
+      simplify with monad laws.
+    finish honing.
+  }
+
+  hone method "YoungOwners'Breeds".
+  {
+    simplify with monad laws; simpl.
+    unfold MyListImpl_abs in *; intuition.
+    rewrite refine_List_Query_In by apply H3.
+    rewrite refine_Join_List_Query_In by apply H0.
+    rewrite refine_List_Query_In_Where.
+    rewrite refine_List_Query_In_Where.
+    rewrite refine_List_For_Query_In_Return;
+      simplify with monad laws; simpl.
+
+    setoid_rewrite refineEquiv_pick_pair_pair.
+    setoid_rewrite refineEquiv_pick_eq'.
+    simplify with monad laws.
+    rewrite refine_pick_val by apply H0.
+    simplify with monad laws.
+    rewrite refine_pick_val by apply H3.
+    simplify with monad laws.
+    rewrite H2.
+    finish honing.
+  }
+
+  hone method "BreedPopulation".
+  {
+    simplify with monad laws; simpl.
+    
+    unfold MyListImpl_abs in *; intuition.
+    setoid_rewrite refineEquiv_pick_pair_pair.
+    setoid_rewrite refineEquiv_pick_eq'.
+    simplify with monad laws.
+    rewrite refine_pick_val by apply H0.
+    simplify with monad laws.
+    rewrite refine_pick_val by apply H3.
+    simplify with monad laws.
+    rewrite H2.
+    finish honing.
+  }
+
+  finish sharpening.
+Defined.
