src/ADTRefinement/BuildADTRefinements/HoneRepresentation.v
@@ -4,6 +4,7 @@ Require Import List Common
         ADTNotation.ilist ADTNotation.StringBound
         ADTRefinement.Core ADTRefinement.SetoidMorphisms
         ADTRefinement.GeneralRefinements
+        ADTRefinement.GeneralBuildADTRefinements
         ADTRefinement.Refinements.HoneRepresentation
         ADTRefinement.BuildADTSetoidMorphisms.
 
@@ -47,15 +48,86 @@ Section HoneRepresentation.
     eapply refineADT_Build_ADT_Rep with (AbsR := AbsR); eauto; intros.
     - unfold getConsDef.
       rewrite <- ith_Bounded_imap.
-      unfold absConsDef, refineConstructor, refine; simpl; intros.
+      unfold absConsDef, absConstructor, refineConstructor, refine; simpl; intros.
       inversion_by computes_to_inv; eauto.
     - unfold getMethDef.
       rewrite <- ith_Bounded_imap.
-      unfold absMethDef, refineMethod, refine; simpl; intros.
+      unfold absMethDef, absMethod, refineMethod, refine; simpl; intros.
       inversion_by computes_to_inv; eauto.
       destruct (H0 _ H) as [or' [Comp_or [AbsR_or'' or''_eq] ] ];
         subst; repeat econstructor; eauto.
       destruct v; simpl in *; subst; econstructor.
+  Qed.
+
+  (* [refine_AbsMethod] can be applied when honing methods to
+     get goals in a nicer form. *)
+
+  Lemma refine_AbsMethod :
+    forall Dom Cod oldMethod nr (d : Dom) refinedMeth,
+      (forall or,
+         AbsR or nr ->
+         refine (or' <- oldMethod or d;
+                 nr' <- { nr' | AbsR (fst or') nr'};
+                 ret (nr', snd or'))
+                (refinedMeth nr d))
+      -> refine (absMethod (Cod := Cod) AbsR oldMethod nr d)
+                (refinedMeth nr d).
+  Proof.
+    unfold absMethod, refine; intros * H v ComputesTo_v; econstructor;
+    intros or AbsR_or.
+    pose proof (H _ AbsR_or v ComputesTo_v); inversion_by computes_to_inv;
+    subst.
+    eexists; split; eauto.
+  Qed.
+
+  Lemma refine_AbsMethod' :
+    forall Dom Cod oldMethod nr (d : Dom) refinedMeth,
+      refine (absMethod (Cod := Cod) AbsR oldMethod nr d)
+             (refinedMeth nr d)
+      -> (forall or,
+            AbsR or nr ->
+            refine (or' <- oldMethod or d;
+                    nr' <- { nr' | AbsR (fst or') nr'};
+                    ret (nr', snd or'))
+                   (refinedMeth nr d)).
+  Proof.
+    unfold absMethod, refine; intros * H or AbsR_or v ComputesTo_v.
+    pose proof (H v ComputesTo_v); inversion_by computes_to_inv;
+    subst.
+    destruct (H0 _ AbsR_or); intuition; subst.
+    repeat econstructor; eauto.
+    rewrite H4; destruct v; econstructor.
+  Qed.
+
+  (* [refine_AbsConstructor] can be applied when honing constructors to
+     get goals in a nicer form. *)
+
+  Lemma refine_AbsConstructor :
+    forall Dom oldConstructor (d : Dom) refinedConstructor,
+      (refine (or' <- oldConstructor d;
+               { nr' | AbsR or' nr'})
+                (refinedConstructor d))
+      -> refine (absConstructor AbsR oldConstructor d)
+                (refinedConstructor d).
+  Proof.
+    unfold absConstructor, refine; intros * H v ComputesTo_v; econstructor.
+    pose proof (H v ComputesTo_v); inversion_by computes_to_inv;
+    subst.
+    eexists; split; eauto.
+  Qed.
+
+  Lemma refine_AbsConstructor' :
+    forall Dom oldConstructor (d : Dom) refinedConstructor,
+      refine (absConstructor AbsR oldConstructor d)
+             (refinedConstructor d)
+      -> (refine (or' <- oldConstructor d;
+                  { nr' | AbsR or' nr'})
+                 (refinedConstructor d)).
+  Proof.
+    unfold absConstructor, refine; intros * H v ComputesTo_v.
+    pose proof (H v ComputesTo_v); inversion_by computes_to_inv;
+    subst.
+    repeat econstructor; eauto.
   Qed.
 
 End HoneRepresentation.
@@ -66,5 +138,98 @@ End HoneRepresentation.
 Tactic Notation "hone" "representation" "using" open_constr(AbsR') :=
   eapply SharpenStep;
   [eapply refineADT_BuildADT_Rep_default with (AbsR := AbsR') |
-   compute [imap absConsDef absConstructor
-                 absMethDef absMethod]; simpl ].
+   compute [imap absConsDef absMethDef]; simpl ].
+
+Tactic Notation "hone" "constructor" constr(consIdx) :=
+  let A :=
+      match goal with
+          |- Sharpened ?A => constr:(A) end in
+  let ASig := match type of A with
+                  ADT ?Sig => Sig
+              end in
+  let consSigs :=
+      match ASig with
+          BuildADTSig ?consSigs _ => constr:(consSigs) end in
+  let methSigs :=
+      match ASig with
+          BuildADTSig _ ?methSigs => constr:(methSigs) end in
+  let consDefs :=
+      match A with
+          BuildADT ?consDefs _  => constr:(consDefs) end in
+  let methDefs :=
+      match A with
+          BuildADT _ ?methDefs  => constr:(methDefs) end in
+  let Rep' :=
+      match A with
+          @BuildADT ?Rep _ _ _ _ => constr:(Rep) end in
+  let ConstructorIndex' := eval simpl in (ConstructorIndex ASig) in
+  let MethodIndex' := eval simpl in (MethodIndex ASig) in
+  let ConstructorDom' := eval simpl in (ConstructorDom ASig) in
+  let consIdxB := eval simpl in
+  (@Build_BoundedIndex _ (List.map consID consSigs) consIdx _) in
+      eapply (@SharpenStep_BuildADT_ReplaceConstructor_eq
+               Rep'  _ _ consDefs methDefs consIdxB
+               (@Build_consDef Rep'
+                              {| consID := consIdx;
+                                 consDom := ConstructorDom' consIdxB
+                              |}
+                              _
+             ));
+    [ intros; simpl in *; set_evars; simpl in *;
+      match goal with
+        |  |- refine (absConstructor ?AbsR ?oldConstructor ?d)
+                     (?H ?d) =>
+           eapply (@refine_AbsConstructor _ _ AbsR _ oldConstructor)
+        | _ => cbv [absConstructor]
+      end
+    |  cbv beta in *; simpl in *;
+       cbv beta delta [replace_BoundedIndex replace_Index] in *;
+       simpl in *].
+
+Tactic Notation "hone" "method" constr(methIdx) :=
+  let A :=
+      match goal with
+          |- Sharpened ?A => constr:(A) end in
+  let ASig := match type of A with
+                  ADT ?Sig => Sig
+              end in
+  let consSigs :=
+      match ASig with
+          BuildADTSig ?consSigs _ => constr:(consSigs) end in
+  let methSigs :=
+      match ASig with
+          BuildADTSig _ ?methSigs => constr:(methSigs) end in
+  let consDefs :=
+      match A with
+          BuildADT ?consDefs _  => constr:(consDefs) end in
+  let methDefs :=
+      match A with
+          BuildADT _ ?methDefs  => constr:(methDefs) end in
+  let Rep' :=
+      match A with
+          @BuildADT ?Rep _ _ _ _ => constr:(Rep) end in
+  let ConstructorIndex' := eval simpl in (ConstructorIndex ASig) in
+  let MethodIndex' := eval simpl in (MethodIndex ASig) in
+  let MethodDomCod' := eval simpl in (MethodDomCod ASig) in
+  let methIdxB := eval simpl in
+  (@Build_BoundedIndex _ (List.map methID methSigs) methIdx _) in
+      eapply (@SharpenStep_BuildADT_ReplaceMethod_eq
+                Rep'  _ _ consDefs methDefs methIdxB
+                (@Build_methDef Rep'
+                               {| methID := methIdx;
+                                  methDom := fst (MethodDomCod' methIdxB);
+                                  methCod := snd (MethodDomCod' methIdxB)
+                               |}
+                               _
+                              ));
+    [ intros;
+      simpl in *; set_evars; simpl in *;
+      match goal with
+        |  |- refine (absMethod ?AbsR ?oldMethod ?nr ?d)
+                     (?H ?nr ?d) => eapply (@refine_AbsMethod _ _ AbsR _ _ oldMethod)
+        | _ => cbv [absMethod]
+      end; intros
+    |
+    cbv beta in *; simpl in *;
+    cbv beta delta [replace_BoundedIndex replace_Index] in *;
+    simpl in *].
