src/QueryStructure/Refinements/GeneralQueryStructureRefinements.v
@@ -17,17 +17,59 @@ Ltac pose_string_ids :=
              set (String R R') as str in *
          end.
 
+Lemma Constructor_DropQSConstraints {MySchema} {Dom}
+: forall oldConstructor (d : Dom),
+    refine
+      (or' <- oldConstructor d;
+       {nr' |
+          DropQSConstraints_AbsR (qsSchema := MySchema) or' nr'})
+        (or' <- oldConstructor d;
+         ret (DropQSConstraints or')).
+Proof.
+  unfold refine; intros; inversion_by computes_to_inv.
+  repeat econstructor; eauto.
+Qed.
+
+(* Queries over an empty relation return empty lists. *)
+Lemma refine_For_In_Empty  :
+  forall ResultT MySchema R bod,
+    refine (Query_For (@UnConstrQuery_In ResultT MySchema
+                                   (DropQSConstraints (QSEmptySpec MySchema))
+                                   R bod))
+           (ret []).
+Proof.
+  intros; rewrite refine_For.
+  simplify with monad laws.
+  unfold In, DropQSConstraints, GetUnConstrRelation in *.
+  rewrite <- ith_Bounded_imap.
+  unfold QSEmptySpec; simpl rels.
+  rewrite Build_EmptyRelation_IsEmpty; simpl.
+  rewrite refine_pick_val with
+  (A := list (IndexedTuple)) (a := [])
+    by (repeat econstructor; eauto).
+  simplify with monad laws.
+  rewrite refine_pick_val with
+  (A := list ResultT) (a := []); reflexivity.
+Qed.
+
 Tactic Notation "start" "honing" "QueryStructure" :=
   pose_string_ids;
   match goal with
       |- context [@BuildADT (QueryStructure ?Rep) _ _ _ _] =>
       hone representation using (@DropQSConstraints_AbsR Rep);
-        repeat (pose_string_ids;
-                match goal with
-                    |- context [(meth ?R (_ : rep , _ : _ ) : _ :=
-                                   {_ | forall or : QueryStructure _,
-                                          DropQSConstraints_AbsR or _ -> _})%methDef] =>
-                    first [ drop constraints from query R
-                          | drop constraints from insert R ]
-                end)
-    end.
+        match goal with
+            |- context [Build_consDef (@Build_consSig ?Id _)
+                                      (@absConstructor _ _ _ _ _)] =>
+            hone constructor Id;
+              [ etransitivity;
+                [apply Constructor_DropQSConstraints |
+                 simplify with monad laws; finish honing]
+              | ]
+        end; pose_string_ids;
+        repeat (match goal with
+                    |- context [Build_methDef (@Build_methSig ?Id _ _)
+                                              (@absMethod _ _ _ _ _ _)] =>
+                    first [ drop constraints from query Id
+                          | drop constraints from insert Id ]
+                end; pose_string_ids)
+  end.
